theories/L6_PCPS/hoare.v
@@ -1,0 +1,139 @@
+Require Import ExtLib.Structures.Monads ExtLib.Data.Monads.StateMonad.
+Import MonadNotation.
+
+Definition triple {A S} (pre : S -> Prop) (e : state S A)
+           (post : S -> A -> S -> Prop) : Prop :=
+  forall i, pre i ->
+       let (v, i') := runState e i in
+       post i v i'.
+
+Notation "{{ p }} e {{ q }}" :=
+  (triple p e q) (at level 90, e at next level).
+
+Lemma return_triple {A S} (x : A) (Pre : S -> Prop) (Post : S -> A -> S -> Prop) :
+  (forall i, Pre i -> Post i x i) ->
+  {{ Pre }} (ret x) {{ Post }}.
+Proof.
+  unfold triple. auto.
+Qed.
+
+Lemma bind_triple {A B S} (m : state S A) (f : A -> state S B)
+      (pre : S -> Prop) (post : S -> B -> S -> Prop)
+      (post' : S -> A -> S -> Prop):
+  {{ pre }} m {{ post' }} ->
+  (forall (x : A) i, {{ post' i x }} f x {{ fun i' => post i }}) -> 
+  {{ pre }} bind m f {{ post }}.
+Proof.
+  simpl. unfold triple; simpl. 
+  intros H1 H2 i Pre.
+  destruct (runState m i) eqn:Heq. eapply H2.
+  specialize (H1 i). rewrite Heq in H1. eapply H1; eauto.
+Qed.
+
+Lemma pre_strenghtening {A S} (P P' : S -> Prop) (Q : S -> A -> S -> Prop) e :  
+  (forall i, P' i -> P i) ->
+  {{ P }} e {{ Q }} ->
+  {{ P' }} e {{ Q }}.
+Proof.
+  intros H. unfold triple. intros; eauto. eapply H0. eauto.
+Qed.
+
+Lemma post_weakening {A S} (P : S -> Prop) (Q Q' : S -> A -> S -> Prop) e :  
+  (forall i x i', P i -> Q i x i' -> Q' i x i') ->
+  {{ P }} e {{ Q }} ->
+  {{ P }} e {{ Q' }}.
+Proof.
+  intros H. unfold triple. intros.
+  specialize (H0 i). destruct (runState e i). eapply H; eauto.
+Qed.
+
+Lemma pre_post_mp_l {A S} (P : S -> Prop) (Q : S -> A -> S -> Prop) e:
+  {{ fun i => True }} e {{ fun i x i' => P i -> Q i x i' }} ->
+  {{ fun i => P i }} e {{ fun i x i' => Q i x i' }}.
+Proof.
+  intros H.
+  eapply post_weakening; [| eapply pre_strenghtening; [| eassumption ] ];
+  simpl; eauto. 
+Qed.
+
+Lemma pre_post_mp_r {A S} (P : S -> Prop) (Q : S -> A -> S -> Prop) e:
+  {{ fun i => P i }} e {{ fun i x i' => Q i x i' }} ->
+  {{ fun i => True }} e {{ fun i x i' => P i -> Q i x i' }}.
+Proof.
+  unfold triple.
+  intros H i HP'. specialize (H i). destruct (runState e i) as [x i'].
+  eauto.
+Qed.
+
+Lemma pre_eq_state {A S} (P : S -> Prop) (Q : S -> A -> S -> Prop) e :
+  (forall i, P i -> {{ fun i' => i = i' }} e {{ Q }}) ->
+  {{ P }} e {{ Q }}.
+Proof.
+  intros H i HP. specialize (H i HP). 
+  unfold triple in H. eapply H. eauto. 
+Qed.
+
+Lemma post_conj {A S} (P : S -> Prop) (Q1 Q2 : S -> A -> S -> Prop) e :
+  {{ P }} e {{ Q1 }} ->
+  {{ P }} e {{ Q2 }} ->
+  {{ P }} e {{ fun i x i' => Q1 i x i' /\ Q2 i x i' }}.
+Proof.
+  unfold triple. intros.
+  specialize (H i); specialize (H0 i).
+  destruct (runState e i); eauto.
+Qed.
+
+Lemma post_trivial { A S} (P : S -> Prop)  (e : state S A) :
+  {{ P }} e {{ fun _ _ _ => True }}.
+Proof.
+  unfold triple. intros; destruct (runState _ _); eauto.
+Qed.
+
+Lemma frame_rule { A S} (Pre : S -> Prop) (Post : S -> A -> S -> Prop)
+      (P : S -> Prop) (e : state S A) :
+  {{ Pre }} e {{ Post }} ->
+  {{ fun i => P i /\ Pre i }} e {{ fun i x i' => P i /\ Post i x i' }}.
+Proof.
+  unfold triple. intros.
+  specialize (H i). destruct (runState _ _). destruct H0; split; eauto.
+Qed.
+
+
+Lemma frame_rule_trivial_pre { A S} (Post : S -> A -> S -> Prop)
+      (P : Prop) (e : state S A) :
+  (P -> {{ fun _ => True }} e {{ Post }}) ->
+  {{ fun i => P }} e {{ fun i x i' => P /\ Post i x i' }}.
+Proof.
+  intros H. unfold triple in *; intros. specialize (H H0 i).
+  destruct (runState e i); split; eauto. 
+Qed.
+
+Lemma frame_rule_trivial { A S} (P : S -> Prop) (e : state S A) :
+  {{ fun i => P i }} e {{ fun i _ _ => P i }}.
+Proof.
+  eapply post_weakening; [| eapply pre_strenghtening;
+                            [| eapply frame_rule with (Pre := (fun _ => True));
+                               eapply post_trivial]]; simpl in *.
+  intros. destruct H0; eauto.
+  intros; eauto.
+Qed.
+
+Lemma get_triple {S} :
+  {{ fun (i : S) => True }}
+    get
+  {{ fun (i : S) (x : S) (i' : S) =>
+       x = i /\ i = i' }}.
+Proof.
+  unfold triple; intros. simpl. eauto.
+Qed.
+
+Lemma put_triple {S} x :
+  {{ fun (i : S) => True }}
+    put x
+  {{ fun (_ : S) (_ : unit) (i' : S) =>
+       x = i' }}.
+Proof.
+  unfold triple; intros. simpl. eauto.
+Qed.
+
+Opaque triple bind ret.
